CL comment fixes and general clean up things.
1. Finished the coordinated close example
2. Fixed type class plumbing
3. Added some comments for the chan record
4. Added an init file so that the package init isn't duplicated
5. Made a class for all the ghost state.

new/proof/github_com/goose_lang/goose/model/channel/chan_spec_inv.v
@@ -6,81 +6,88 @@ Require Import New.proof.sync.
 
 Section proof.
  Context `{hG: heapGS Σ, !ffi_semantics _ _}. 
-Context `{!closePropTrackerG Σ,  !inG Σ (authR (optionUR (prodR fracR natR)))}.
+Context  `{!chanGhostStateG Σ}.
 
-Implicit Types (v:val). 
-Context `{!ghost_varG Σ (bool * val)}.
-
-
-
-Record chan  (t': Type) := {
-  ch_T: go_type;
-  #[export]
-  ch_IntoVal:: IntoVal t';
-  #[export]
-  ch_IntoValTyped:: IntoValTyped t' ch_T;
-  #[export]
-  ch_Hbounded:: BoundedTypeSize ch_T;
+Record chan  (V: Type )  := {
+  (* Type and type classes for the value type of a channel *)
+  ch_t : go_type;
+  ch_IntoVal : IntoVal V;
+  ch_IntoValTyped : IntoValTyped V ch_t;
+  ch_BoundedTypeSize : BoundedTypeSize ch_t;
+  (* ptr to channel *)
   ch_loc: loc;
+  (* mutex that guards channel internals *)
   ch_mu: loc;
+  (* slice that acts as buffered channel's internal circular buffer *)
   ch_buff: slice.t;
+  (* ghost names for channel ghost state *)
   ch_γ: chan_names;
+  (* 0 for unbuffered, size of buffer for buffered *)
   ch_size: Z;
+  (* 
+    Whether this channel will only be used by 1 sender and 1 receiver. If so, we 
+    can access the sequence number in predicates using the _single versions below
+  *)
   ch_is_single_party: bool;
-  ch_q: Qp;
-  ch_Psingle: Z -> t' -> iProp Σ;
-  ch_Pmulti: t' -> iProp Σ;
+  (* Predicates sent from sender to receiver, where we can access the sequence 
+    number if we agree not to have multiple parties, which loses ordering.
+
+    If you aren't planning on using this predicate, just have it return True or emp. If 
+    you are planning on restricting the number of operations over the channel to n, 
+    have it return False after n operations
+  *)
+  ch_Psingle: Z -> V -> iProp Σ;
+  ch_Pmulti: V -> iProp Σ;
+  (* Predicates sent from receiver to sender, where we can access the sequence 
+    number if we agree not to have multiple parties, which loses ordering. 
+    ch_Qsingle handles buffered channels by allowing a sender to gain the i-buffer_size 
+    predicate, providing synchronization by guaranteeing a receiver has blocked or 
+    consumed a value. 
+
+    If you aren't planning on using this predicate, just have it return True or emp. If 
+    you are planning on restricting the number of operations over the channel to n, 
+    have it return False after n operations
+  *)
   ch_Qsingle: Z -> iProp Σ;
   ch_Qmulti: iProp Σ;
+  (* 
+    The central predicate for closing. The nat here is the number of sends/receives at 
+    the time of close. If we won't close, use (n) => False 
+    This can be split amongst multiple receivers using the lemmas in chan_ghost_state.
+   *)
   ch_R: nat -> iProp Σ;
 }.
-  Arguments ch_T {t'}.
-  Arguments ch_IntoVal {t'}.
-Arguments ch_T {t'} .
-Arguments ch_IntoVal {t'} .
-Arguments ch_IntoValTyped {t'} .
-Arguments ch_Hbounded {t'} .
-Arguments ch_loc {t'} .
-Arguments ch_mu {t'} .
-Arguments ch_buff {t'} .
-Arguments ch_γ {t'} .
-Arguments ch_size {t'} .
-Arguments ch_is_single_party {t'} .
-Arguments ch_q {t'} .
-Arguments ch_Psingle {t'} .
-Arguments ch_Pmulti {t'} .
-Arguments ch_Qsingle {t'} .
-Arguments ch_Qmulti {t'} .
 
-
+Arguments ch_loc: default implicits.
+Arguments ch_mu: default implicits.
+Arguments ch_buff: default implicits.
+Arguments ch_γ: default implicits.
+Arguments ch_size: default implicits.
+Arguments ch_is_single_party: default implicits.
+Arguments ch_Psingle: default implicits.
+Arguments ch_Qsingle: default implicits.
+Arguments ch_Qmulti: default implicits.
+Arguments ch_Pmulti: default implicits.
+Arguments ch_R: default implicits.
 
 (* Args for a simple use of send for synchronization i.e. using Send to join a goroutine. 
  Enforces that a channel isn't closed using a always-False R predicate. 
  *)
 Definition make_unbuffered_params_simple_single_sync
- (t': Type)
-(t: go_type)
-(iv: IntoVal t')
-(ivt: IntoValTyped t' t)
-(hb: BoundedTypeSize t)
+V {H: IntoVal V} {t} {H': IntoValTyped V t} {B: BoundedTypeSize t}
 (ch: loc)
 (mu: loc)
 (buff: slice.t)
 (γ: chan_names)
-(Psingle: Z -> t' -> iProp Σ)
-: chan t' :=
+(Psingle: Z -> V -> iProp Σ)
+: chan V :=
 {|
-  ch_T := t;
-  ch_IntoVal := iv;
-  ch_IntoValTyped := ivt;
-  ch_Hbounded := hb;
   ch_loc := ch;
   ch_mu := mu;
   ch_buff := buff;
   ch_γ := γ;
   ch_size := 0;
   ch_is_single_party := true;
-  ch_q := 1%Qp;
   ch_Psingle := Psingle;  
   ch_Pmulti := λ _, True%I;    
   ch_Qsingle := λ _, True%I;   
@@ -89,12 +96,11 @@ Definition make_unbuffered_params_simple_single_sync
 |}
 .
 
-
-Definition P {T'} (is_single_party: bool) (i: Z) (v: T') 
-              (Psingle: Z -> T' -> iProp Σ) (Pmulti: T' -> iProp Σ) : iProp Σ := 
+Definition P (V: Type) {H: IntoVal V} {t} {H': IntoValTyped V t} (is_single_party: bool) (i: Z) (v: V) 
+              (Psingle: Z -> V -> iProp Σ) (Pmulti: V -> iProp Σ) : iProp Σ := 
   if is_single_party then Psingle i v else Pmulti v.
 
-Definition Q (is_single_party: bool) (z: Z) 
+Definition Q (V: Type) {H: IntoVal V} {t} {H': IntoValTyped V t} (is_single_party: bool) (z: Z) 
               (Qsingle: Z -> iProp Σ) (Qmulti: iProp Σ) : iProp Σ := 
   if bool_decide(Z.lt z 0%Z) then True%I else (if is_single_party then Qsingle(z) else Qmulti).
 
@@ -102,33 +108,28 @@ Definition buff_size_inv (count : Z) (first : u64) (size : Z): iProp Σ :=
 (⌜count <= size⌝ ∗ ⌜word.unsigned first < size⌝ ∗ ⌜size > 0⌝ ∗ ⌜size + 1 < 2 ^ 63⌝
 ∗ ⌜count + 1 < 2 ^ 63⌝)%I.
 
-Definition valid_elems {T'} (slice : list T') (first : u64) (count : u64) : list T' :=
+Definition valid_elems (V: Type) (slice : list V) (first : u64) (count : u64) : list V :=
   subslice (uint.nat first) (uint.nat first + uint.nat count) (slice ++ slice).
 
-Definition isBufferedChanLogical  {t': Type} 
- (params: chan t'  ) 
+Definition isBufferedChanLogical (V: Type) {H: IntoVal V} {t} {H': IntoValTyped V t}
+ (params: chan V  ) 
   (vs: valid_chan_state) (send_count recv_count: nat) (count: Z) 
-  (first: u64) (xs: list t') : iProp Σ := 
+  (first: u64) (xs: list V) : iProp Σ := 
   "%HCountMinus" ∷ ⌜count = (send_count - recv_count)⌝ ∗
-  "%HSizeLen" ∷ ⌜ch_size params = length xs⌝ ∗
+  "%HSizeLen" ∷ ⌜(ch_size params) = length xs⌝ ∗
   "%HBuffSizeInv" ∷ buff_size_inv count first (length xs) ∗
-  "HPs" ∷ ([∗ list] i↦x ∈ valid_elems xs first count, 
-            P params.(ch_is_single_party)  (recv_count + i) x params.(ch_Psingle) params.(ch_Pmulti)) ∗ 
-  "HQs" ∷ big_sep_seq send_count (params.(ch_size)- count) 
-           (λ i, Q (ch_is_single_party  params) (i - params.(ch_size)) params.(ch_Qsingle) params.(ch_Qmulti)).
+  "HPs" ∷ ([∗ list] i↦x ∈ valid_elems V xs first count, 
+            P V (ch_is_single_party params)  (recv_count + i) x (ch_Psingle params) (ch_Pmulti   params)) ∗ 
+  "HQs" ∷ big_sep_seq send_count ((ch_size params)- count) 
+           (λ i, Q V (ch_is_single_party params) (i - (ch_size params)) (ch_Qsingle  params) (ch_Qmulti params)).
 
-Definition isBufferedChan (t': Type)  (params: chan t' ) 
+Definition isBufferedChan (V: Type) {H: IntoVal V} {t} {H': IntoValTyped V t}  (params: chan V ) 
   (vs: valid_chan_state) (send_count recv_count: nat) (count: Z) 
   (first: u64) : iProp Σ := 
-  let intoVal := params.(ch_IntoVal) in
-  let T := params.(ch_T) in
-  let IntoVal_inst := params.(ch_IntoVal) in
-  let IntoValTyped_inst := params.(ch_IntoValTyped) in
-  let Hbounded := params.(ch_Hbounded) in
-  ∃ (xs: list t'), 
+  ∃ (xs: list V), 
     "HBuffSlice" ∷ own_slice 
-                     params.(ch_buff) (DfracOwn 1) xs ∗
-    isBufferedChanLogical params vs send_count recv_count count first xs.
+                     (ch_buff params) (DfracOwn 1) xs ∗
+    isBufferedChanLogical V params vs send_count recv_count count first xs.
 
 Definition chan_state_facts (vs: valid_chan_state) (send_count recv_count: nat) : iProp Σ :=
 match vs with
@@ -140,40 +141,39 @@ match vs with
   | Valid_closed => ⌜send_count = recv_count⌝
 end.
 
-Definition chan_state_resources (t': Type) (params: chan t')
-  (vs: valid_chan_state) (send_count recv_count: nat) (v: t') : iProp Σ :=
-    let _ : IntoVal t' := params.(ch_IntoVal) in
+Definition chan_state_resources (V: Type) {H: IntoVal V} {t} {H': IntoValTyped V t} (params: chan V)
+  (vs: valid_chan_state) (send_count recv_count: nat) (v: V) : iProp Σ :=
   match vs with
   | Valid_start => 
-      "Hextok" ∷ full_exchange_token params.(ch_γ)
+      "Hextok" ∷ full_exchange_token (ch_γ params)
   | Valid_receiver_ready => 
       "Hextok" ∷ receiver_exchange_token params.(ch_γ) ∗
-      "HQ" ∷ Q params.(ch_is_single_party) recv_count params.(ch_Qsingle) params.(ch_Qmulti)
+      "HQ" ∷ Q V params.(ch_is_single_party) recv_count params.(ch_Qsingle) params.(ch_Qmulti)
   | Valid_sender_ready => 
       "Hextok" ∷ sender_exchange_token params.(ch_γ) v ∗
-      "HP" ∷ P params.(ch_is_single_party) send_count v params.(ch_Psingle) params.(ch_Pmulti)
+      "HP" ∷ P V (ch_is_single_party params) send_count v params.(ch_Psingle) (ch_Pmulti params)
   | Valid_receiver_done => 
       "Hextok" ∷ sender_exchange_token params.(ch_γ) v ∗
-      "HQ" ∷ Q params.(ch_is_single_party) send_count params.(ch_Qsingle) params.(ch_Qmulti)
+      "HQ" ∷ Q V params.(ch_is_single_party) send_count params.(ch_Qsingle) params.(ch_Qmulti)
   | Valid_sender_done => 
       "Hextok" ∷ receiver_exchange_token params.(ch_γ) ∗
-      "HP" ∷ P params.(ch_is_single_party) recv_count v params.(ch_Psingle) params.(ch_Pmulti)
+      "HP" ∷ P V params.(ch_is_single_party) recv_count v params.(ch_Psingle) (ch_Pmulti params)
   | Valid_closed => emp
   end.
 
 
-Definition isUnbufferedChan (t': Type) (params: chan t')
-(v: t') (vs: valid_chan_state) (send_count recv_count: nat) : iProp Σ := 
+Definition isUnbufferedChan (V: Type) {H: IntoVal V} {t} {H': IntoValTyped V t} (params: chan V)
+(v: V) (vs: valid_chan_state) (send_count recv_count: nat) : iProp Σ := 
 "%HUnBuffFacts" ∷ chan_state_facts vs send_count recv_count ∗
-chan_state_resources t' params vs send_count recv_count v.
+chan_state_resources V params vs send_count recv_count v.
 
-Definition isChanInner (t': Type) (params: chan t'): iProp Σ := 
-  ∃ (vs: valid_chan_state) (count: nat) (first: u64) (v: t') (send_count recv_count: nat),
+Definition isChanInner (V: Type) {H: IntoVal V} {t} {H': IntoValTyped V t} (params: chan V): iProp Σ := 
+  ∃ (vs: valid_chan_state) (count: nat) (first: u64) (v: V) (send_count recv_count: nat),
     (* Physical state *)
-    "value" ∷ params.(ch_loc) ↦s[(channel.Channel.ty params.(ch_T)) :: "v"] v ∗ 
-    "first" ∷ params.(ch_loc) ↦s[(channel.Channel.ty params.(ch_T)) :: "first"] first ∗
-    "count" ∷ params.(ch_loc) ↦s[(channel.Channel.ty params.(ch_T)) :: "count"] (W64 count) ∗ 
-    "state" ∷ params.(ch_loc) ↦s[(channel.Channel.ty params.(ch_T)) :: "state"] (valid_to_word vs) ∗ 
+    "value" ∷ params.(ch_loc) ↦s[(channel.Channel.ty t) :: "v"] v ∗ 
+    "first" ∷ params.(ch_loc) ↦s[(channel.Channel.ty t) :: "first"] first ∗
+    "count" ∷ params.(ch_loc) ↦s[(channel.Channel.ty t) :: "count"] (W64 count) ∗ 
+    "state" ∷ params.(ch_loc) ↦s[(channel.Channel.ty t) :: "state"] (valid_to_word vs) ∗ 
     
     (* Counter resources *)
     "HSndCtrAuth" ∷ own_send_counter_auth params.(ch_γ) send_count (send_ctr_frozen vs) ∗ 
@@ -192,18 +192,18 @@ Definition isChanInner (t': Type) (params: chan t'): iProp Σ :=
     (* Buffer vs unbuffered channels *)
     "HChanState" ∷ 
       (if params.(ch_size) =? 0 then
-        isUnbufferedChan t' params v vs send_count recv_count
+        isUnbufferedChan V params v vs send_count recv_count
       else
-        isBufferedChan t' params vs send_count recv_count count first).
+        isBufferedChan V params vs send_count recv_count count first).
 
-Definition isChanInnerClosed (params: chan t'): iProp Σ := 
+Definition isChanInnerClosed (V: Type) {H: IntoVal V} {t} {H': IntoValTyped V t} (params: chan V): iProp Σ := 
 
-  ∃ (count: nat) (first: u64) (v: t') (send_count recv_count: nat),
+  ∃ (count: nat) (first: u64) (v: V) (send_count recv_count: nat),
     (* Physical state *)
-    "value" ∷ params.(ch_loc) ↦s[(channel.Channel.ty T) :: "v"] v ∗ 
-    "first" ∷ params.(ch_loc) ↦s[(channel.Channel.ty T) :: "first"] first ∗
-    "count" ∷ params.(ch_loc) ↦s[(channel.Channel.ty T) :: "count"] (W64 count) ∗ 
-    "state" ∷ params.(ch_loc) ↦s[(channel.Channel.ty T) :: "state"] (valid_to_word Valid_closed) ∗ 
+    "value" ∷ params.(ch_loc) ↦s[(channel.Channel.ty t) :: "v"] v ∗ 
+    "first" ∷ params.(ch_loc) ↦s[(channel.Channel.ty t) :: "first"] first ∗
+    "count" ∷ params.(ch_loc) ↦s[(channel.Channel.ty t) :: "count"] (W64 count) ∗ 
+    "state" ∷ params.(ch_loc) ↦s[(channel.Channel.ty t) :: "state"] (valid_to_word Valid_closed) ∗ 
     
     (* Counter resources *)
     "HSndCtrAuth" ∷ own_send_counter_auth params.(ch_γ) send_count (send_ctr_frozen Valid_closed) ∗ 
@@ -220,104 +220,103 @@ Definition isChanInnerClosed (params: chan t'): iProp Σ :=
     (* Buffer vs unbuffered channels *)
     "HChanState" ∷ 
       (if params.(ch_size) =? 0 then
-        isUnbufferedChan params v Valid_closed send_count recv_count
+        isUnbufferedChan V params v Valid_closed send_count recv_count
       else
-        isBufferedChan params Valid_closed send_count recv_count count first).
+        isBufferedChan V params Valid_closed send_count recv_count count first).
 
-Definition isChan (params: chan t') : iProp Σ := 
-    "#mu" ∷ params.(ch_loc) ↦s[(channel.Channel.ty T) :: "lock"]□ params.(ch_mu) ∗
-    "#buffer" ∷ params.(ch_loc) ↦s[(channel.Channel.ty T) :: "buffer"]□ params.(ch_buff) ∗
+Definition isChan (V: Type) {H: IntoVal V} {t} {H': IntoValTyped V t} (params: chan V) : iProp Σ := 
+    "#mu" ∷ params.(ch_loc) ↦s[(channel.Channel.ty t) :: "lock"]□ params.(ch_mu) ∗
+    "#buffer" ∷ params.(ch_loc) ↦s[(channel.Channel.ty t) :: "buffer"]□ params.(ch_buff) ∗
     "%Hbuffsize" ∷ ⌜#params.(ch_buff).(slice.len_f) = #(W64 params.(ch_size))⌝ ∗
     "%Hbuffsize" ∷ ⌜0 ≤  params.(ch_size)⌝ ∗
     "%Hbuffsize" ∷ ⌜params.(ch_size) + 1 < 2 ^ 63⌝ ∗
-    "#Hlock" ∷ is_Mutex params.(ch_mu) (isChanInner params).
+    "#Hlock" ∷ is_Mutex params.(ch_mu) (isChanInner V params).
 
-Definition send_pre (params: chan t') (i: nat) (v: t') : iProp Σ :=
+Definition send_pre (V: Type) {H: IntoVal V} {t} {H': IntoValTyped V t} (params: chan V) (q: Qp) (i: nat) (v: V) : iProp Σ :=
   "%HChNonnull" ∷ ⌜params.(ch_loc) ≠ null⌝ ∗
-  "%Hsp" ∷ ⌜if params.(ch_is_single_party) then params.(ch_q) = 1%Qp else (params.(ch_q) < 1)%Qp⌝ ∗
-  "HCh" ∷ isChan params ∗
-  "HP" ∷ P params.(ch_is_single_party) i v params.(ch_Psingle) params.(ch_Pmulti) ∗ 
-  "HSc" ∷ own_send_counter_frag params.(ch_γ) i params.(ch_q).
+  "%Hsp" ∷ ⌜if params.(ch_is_single_party) then q = 1%Qp else (q ≤ 1)%Qp⌝ ∗
+  "HCh" ∷ isChan V params ∗
+  "HP" ∷ P V (ch_is_single_party params) i v params.(ch_Psingle) params.(ch_Pmulti) ∗ 
+  "HSc" ∷ own_send_counter_frag params.(ch_γ) i q.
 
-Definition send_pre_inner (params: chan t') (i: nat) (v: t') : iProp Σ :=
+Definition send_pre_inner (V: Type) {H: IntoVal V} {t} {H': IntoValTyped V t} (params: chan V) (q: Qp) (i: nat) (v: V) : iProp Σ :=
   "%HChNonnull" ∷ ⌜params.(ch_loc) ≠ null⌝ ∗
-  "%Hsp" ∷ ⌜if params.(ch_is_single_party) then params.(ch_q) = 1%Qp else (params.(ch_q) < 1)%Qp⌝ ∗
-  "HCh" ∷ isChanInner params ∗
+  "%Hsp" ∷ ⌜if params.(ch_is_single_party) then q = 1%Qp else (q ≤ 1)%Qp⌝ ∗
+  "HCh" ∷ isChanInner V params ∗
   "%Hbuffsize" ∷ ⌜params.(ch_buff).(slice.len_f) = (W64 params.(ch_size))⌝ ∗
-    "#buffer" ∷ params.(ch_loc) ↦s[(channel.Channel.ty params.(ch_T)) :: "buffer"]□ params.(ch_buff) ∗
-  "HP" ∷ P params.(ch_is_single_party) i v params.(ch_Psingle) params.(ch_Pmulti) ∗ 
-  "HSc" ∷ own_send_counter_frag params.(ch_γ) i params.(ch_q).
+    "#buffer" ∷ params.(ch_loc) ↦s[(channel.Channel.ty t) :: "buffer"]□ params.(ch_buff) ∗
+  "HP" ∷ P V params.(ch_is_single_party) i v (ch_Psingle params) (ch_Pmulti params) ∗ 
+  "HSc" ∷ own_send_counter_frag params.(ch_γ) i q.
 
-Definition send_post (params: chan t') (i: nat) : iProp Σ :=
-Q params.(ch_is_single_party) (i - params.(ch_size)) params.(ch_Qsingle) params.(ch_Qmulti) ∗ 
-own_send_counter_frag params.(ch_γ) (i + 1)%nat params.(ch_q).
+Definition send_post (V: Type) {H: IntoVal V} {t} {H': IntoValTyped V t} (params: chan V) (q: Qp) (i: nat) : iProp Σ :=
+Q V params.(ch_is_single_party) (i - params.(ch_size)) params.(ch_Qsingle) params.(ch_Qmulti) ∗ 
+own_send_counter_frag params.(ch_γ) (i + 1)%nat q.
 
 
-Definition send_post_inner(params: chan t') (i: nat) : iProp Σ :=
-  "HCh" ∷ isChanInner params ∗
-Q params.(ch_is_single_party) (i - params.(ch_size)) params.(ch_Qsingle) params.(ch_Qmulti) ∗ 
-own_send_counter_frag params.(ch_γ) (i + 1)%nat params.(ch_q).
+Definition send_post_inner (V: Type) {H: IntoVal V} {t} {H': IntoValTyped V t} (params: chan V) (q: Qp) (i: nat) : iProp Σ :=
+  "HCh" ∷ isChanInner V params ∗
+Q V params.(ch_is_single_party) (i - params.(ch_size)) params.(ch_Qsingle) params.(ch_Qmulti) ∗ 
+own_send_counter_frag params.(ch_γ) (i + 1)%nat q.
 
-Definition recv_pre (params: chan t') (i: nat) (Ri: nat -> iProp Σ) : iProp Σ :=
+Definition recv_pre (V: Type) {H: IntoVal V} {t} {H': IntoValTyped V t} (params: chan V) (q: Qp) (i: nat) (Ri: nat -> iProp Σ) : iProp Σ :=
   "%HChnonnull" ∷ ⌜params.(ch_loc) ≠ null⌝ ∗
-  "%Hsp" ∷  ⌜if params.(ch_is_single_party) then params.(ch_q) = 1%Qp else (params.(ch_q) < 1)%Qp⌝ ∗
-  "HCh" ∷ isChan params ∗
-  "HQ" ∷ Q params.(ch_is_single_party) i params.(ch_Qsingle) params.(ch_Qmulti) ∗ 
-  "HRecvPerm" ∷ own_recv_perm params.(ch_γ) params.(ch_q) i Ri.
+  "%Hsp" ∷  ⌜if params.(ch_is_single_party) then q = 1%Qp else (q ≤ 1)%Qp⌝ ∗
+  "HCh" ∷ isChan V params ∗
+  "HQ" ∷ Q V params.(ch_is_single_party) i params.(ch_Qsingle) params.(ch_Qmulti) ∗ 
+  "HRecvPerm" ∷ own_recv_perm params.(ch_γ) q i Ri.
 
-Definition default_val (params: chan t') : t' :=
-@default_val t' params.(ch_T) _ params.(ch_IntoVal) params.(ch_IntoValTyped).
+Definition default_val (V: Type) {H: IntoVal V} {t} {H': IntoValTyped V t} (params: chan V) : V :=
+@default_val V t _ H H'.
 
-Definition recv_post (params: chan t') (i: nat) (ok: bool) (v: t') (Ri: nat -> iProp Σ) : iProp Σ :=
+Definition recv_post (V: Type) {H: IntoVal V} {t} {H': IntoValTyped V t} (params: chan V) (q: Qp) (i: nat) (ok: bool) (v: V) (Ri: nat -> iProp Σ) : iProp Σ :=
 if ok then
-  (P params.(ch_is_single_party) i v params.(ch_Psingle) params.(ch_Pmulti) ∗ 
-   own_recv_perm params.(ch_γ) params.(ch_q) (i + 1) Ri)%I
+  (P V params.(ch_is_single_party) i v params.(ch_Psingle) params.(ch_Pmulti) ∗ 
+   own_recv_perm params.(ch_γ) q (i + 1) Ri)%I
 else
-  ("HRecFrag" ∷ own_recv_counter_frag params.(ch_γ) i params.(ch_q) ∗ 
-   "%Hvdef" ∷ ⌜v = default_val params⌝ ∗ 
+  ("HRecFrag" ∷ own_recv_counter_frag params.(ch_γ) i q ∗ 
+   "%Hvdef" ∷ ⌜v = default_val V params⌝ ∗ 
    (∃ n, "HRi" ∷ Ri n ∗ 
          "#Hsca" ∷ own_send_counter_auth params.(ch_γ) n true ∗ 
          "#Hrca" ∷ own_recv_counter_auth params.(ch_γ) n true))%I.
 
-Definition recv_pre_inner (params: chan t') (i: nat) (Ri: nat -> iProp Σ) : iProp Σ :=
+Definition recv_pre_inner (V: Type) {H: IntoVal V} {t} {H': IntoValTyped V t} (params: chan V) (q: Qp) (i: nat) (Ri: nat -> iProp Σ) : iProp Σ :=
 "%HChnonnull" ∷ ⌜params.(ch_loc) ≠ null⌝ ∗
-"%Hsp" ∷ ⌜if params.(ch_is_single_party) then params.(ch_q) = 1%Qp else (params.(ch_q) < 1)%Qp⌝ ∗
-"HCh" ∷ isChanInner params ∗
+"%Hsp" ∷ ⌜if params.(ch_is_single_party) then q = 1%Qp else (q ≤ 1)%Qp⌝ ∗
+"HCh" ∷ isChanInner V params ∗
 "%Hbuffsize" ∷ ⌜params.(ch_buff).(slice.len_f) = W64 params.(ch_size)⌝ ∗
-"#buffer" ∷ params.(ch_loc) ↦s[(channel.Channel.ty params.(ch_T)) :: "buffer"]□ params.(ch_buff) ∗
-"HQ" ∷ Q params.(ch_is_single_party) (Z.of_nat i) params.(ch_Qsingle) params.(ch_Qmulti) ∗ 
-"HRecvPerm" ∷ own_recv_perm params.(ch_γ) params.(ch_q) i Ri.
+"#buffer" ∷ params.(ch_loc) ↦s[(channel.Channel.ty t) :: "buffer"]□ params.(ch_buff) ∗
+"HQ" ∷ Q V params.(ch_is_single_party) (Z.of_nat i) params.(ch_Qsingle) params.(ch_Qmulti) ∗ 
+"HRecvPerm" ∷ own_recv_perm params.(ch_γ) q i Ri.
        
-Definition recv_post_inner (params: chan t') (i: nat) (ok: bool) (v: t') (Ri: nat -> iProp Σ) : iProp Σ :=
-  "HCh" ∷ isChanInner params ∗
+Definition recv_post_inner (V: Type) {H: IntoVal V} {t} {H': IntoValTyped V t} (params: chan V) (q: Qp) (i: nat) (ok: bool) (v: V) (Ri: nat -> iProp Σ) : iProp Σ :=
+  "HCh" ∷ isChanInner V params ∗
   if ok then
-    (P params.(ch_is_single_party) (Z.of_nat i) v params.(ch_Psingle) params.(ch_Pmulti) ∗ 
-    own_recv_perm params.(ch_γ) params.(ch_q) (i + 1) Ri)%I
+    (P V params.(ch_is_single_party) (Z.of_nat i) v params.(ch_Psingle) params.(ch_Pmulti) ∗ 
+    own_recv_perm params.(ch_γ) q (i + 1) Ri)%I
   else
-    ("HRecFrag" ∷ own_recv_counter_frag params.(ch_γ) i params.(ch_q) ∗ 
-    "%Hvdef" ∷ ⌜v = default_val params⌝ ∗ 
+    ("HRecFrag" ∷ own_recv_counter_frag params.(ch_γ) i q ∗ 
+    "%Hvdef" ∷ ⌜v = default_val V params⌝ ∗ 
     (∃ n, "HRi" ∷ Ri n ∗ 
           "#Hsca" ∷ own_send_counter_auth params.(ch_γ ) n true ∗ 
           "#Hrca" ∷ own_recv_counter_auth params.(ch_γ) n true))%I.
 
-Lemma closed_unbuff_eq (params: chan t') (send_count recv_count: nat) (v: t'):
-  isUnbufferedChan params v Valid_closed send_count recv_count -∗ ⌜send_count = recv_count⌝.
+Lemma closed_unbuff_eq (V: Type) {H: IntoVal V} {t} {H': IntoValTyped V t} (params: chan V) (send_count recv_count: nat) (v: V):
+  isUnbufferedChan V params v Valid_closed send_count recv_count -∗ ⌜send_count = recv_count⌝.
 Proof.
   iIntros "[%Heq _]". iPureIntro. exact Heq.
 Qed.
 
-Lemma chan_pointsto_non_null (lock: loc) (params: chan t'):
-  params.(ch_loc) ↦s[channel.Channel.ty params.(ch_T) :: "lock"]□ lock -∗ ⌜ #params.(ch_loc) ≠ #null ⌝.
+Lemma chan_pointsto_non_null (V: Type) {H: IntoVal V} {t} {H': IntoValTyped V t} (lock: loc) (params: chan V):
+  params.(ch_loc) ↦s[channel.Channel.ty t :: "lock"]□ lock -∗ ⌜ #params.(ch_loc) ≠ #null ⌝.
 Proof.
   iIntros "Hb.a".
   iDestruct (typed_pointsto_not_null with "Hb.a") as %Hnotnull.
   { rewrite go_type_size_unseal. done. }
-  iPureIntro. intro H. subst.
+  iPureIntro. intro H0. subst.
   rewrite struct.field_ref_f_unseal in Hnotnull.
-  rewrite to_val_unseal in H. simpl in H. inversion H. replace (params.(ch_loc)) with null in *. 
+  rewrite to_val_unseal in H0. simpl in H0. inversion H0. replace (params.(ch_loc)) with null in *. 
   simpl in Hnotnull.
   contradiction.
 Qed.
 
 End proof.
-
