new/proof/github_com/goose_lang/goose/model/channel/chan_init.v
@@ -1,0 +1,14 @@
+From New.generatedproof.github_com.goose_lang.goose Require Import model.channel.
+From New.proof Require Import proof_prelude.
+From New.proof.github_com.goose_lang Require Import primitive.
+From New.proof.github_com.goose_lang.std Require Import std_core.
+Require Export New.code.sync.
+Require Export New.generatedproof.sync.
+From New.proof.sync_proof Require Import base mutex sema.
+
+Section proof.
+Context `{hG: heapGS Σ, !ffi_semantics _ _}.  
+Context `{!goGlobalsGS Σ}.
+Context  `{!chanGhostStateG Σ}.
+#[global] Program Instance : IsPkgInit channel := ltac2:(build_pkg_init ()).
+End proof.
