new/proof/github_com/goose_lang/goose/model/channel/chan_spec_api.v
@@ -1,234 +1,314 @@
 From New.proof.github_com.goose_lang Require Import primitive.
 From New.proof.github_com.goose_lang.std Require Import std_core.
-From New.proof.github_com.goose_lang.goose.model.channel Require Import chan_spec_inv chan_spec_select chan_spec_base chan_spec_send.
+From New.proof.github_com.goose_lang.goose.model.channel Require Import chan_ghost_state chan_spec_inv chan_spec_select chan_spec_base chan_spec_send chan_spec_recv.
 From New.generatedproof.github_com.goose_lang.goose Require Import model.channel.
 From New.proof Require Import proof_prelude.
 Require Export New.code.sync.
 Require Export New.generatedproof.sync.
 From New.proof.sync_proof Require Import base mutex sema.
 
-
 Section proof.
-Context `{hG: heapGS Σ, !ffi_semantics _ _}. 
-Context `{!closePropTrackerG Σ,  !inG Σ (authR (optionUR (prodR fracR natR)))}.
-   Context `{!goGlobalsGS Σ}.
-Context `{!ghost_varG Σ (bool * val)}.
-#[global] Program Instance : IsPkgInit channel := ltac2:(build_pkg_init ()).
+Context `{hG: heapGS Σ, !ffi_semantics _ _}.  
+Context  `{!chanGhostStateG Σ}.
+Context `{!goGlobalsGS Σ}.
 
-Lemma wp_Channel__Send  (params: chan) (i: nat) (v: params.(ch_T')):
-(* Could let bindings be implicit args? *)
-  let T' := params.(ch_T') in
-  let T := params.(ch_T) in
-  let IntoVal_inst := params.(ch_IntoVal) in
-  let IntoValTyped_inst := params.(ch_IntoValTyped) in
-  let Hbounded := params.(ch_Hbounded) in
+Arguments ch_loc: default implicits.
+Arguments ch_mu: default implicits.
+Arguments ch_buff: default implicits.
+Arguments ch_γ: default implicits.
+Arguments ch_size: default implicits.
+Arguments ch_is_single_party: default implicits.
+Arguments ch_Psingle: default implicits.
+Arguments ch_Qsingle: default implicits.
+Arguments ch_Qmulti: default implicits.
+Arguments ch_Pmulti: default implicits.
+Arguments ch_R: default implicits.
+
+(*---------------------------------------------------------------------------
+ User must unfold send_post, see chan_spec_inv for definition and descriptions
+ of chan record components
+ ---------------------------------------------------------------------------*)
+Lemma wp_Channel__Send 
+  (V: Type) {K: IntoVal V} {t: go_type}
+  {H': IntoValTyped V t} {B: BoundedTypeSize t}
+  (params: chan V) (i: nat) (q: Qp) (v: V):
   params.(ch_loc) ≠ null ->
-  (if params.(ch_is_single_party) then params.(ch_q) = 1%Qp else (params.(ch_q) < 1)%Qp) ->
-  {{{ is_pkg_init channel ∗ send_pre params i v }}}
-    params.(ch_loc) @ channel @ "Channel'ptr" @ "Send" #T #v 
-  {{{ RET #();
-      send_post params i
-  }}}.
-Proof. 
-  intros HT' HT Hiv_inst Hivt_inst Hb_inst Hnn Hsp. wp_start. wp_auto.   
-  let x := ident:(Φ) in
-  try clear x.
- iNamed "Hpre". wp_if_destruct;first contradiction. wp_auto.
-  wp_apply (wp_NewSendCase with "[HCh HP c HSc]"). 
+  (if params.(ch_is_single_party) then q = 1%Qp else (q ≤ 1)%Qp) ->
+  {{{ is_pkg_init channel ∗ send_pre V params q i v }}}
+    params.(ch_loc) @ channel @ "Channel'ptr" @ "Send" #t #v 
+  {{{ RET #(); send_post V params q i }}}.
+Proof.
+  intros Hnn Hsp.
+  wp_start. wp_auto.
+  let x := ident:(Φ) in try clear x.
+  iNamed "Hpre".
+  wp_if_destruct; first contradiction.
+  wp_auto.
+  wp_apply (wp_NewSendCase with "[HCh HP c HSc]"). all: try done.
   {
-    iFrame. iPureIntro. done.
+    rewrite -> bool_decide_true by done.
+    iFrame. done.
   }
-  iIntros (case_ptr) "Hosc". wp_auto. wp_apply (wp_Select1 with "[Hosc]").
+  iIntros (case_ptr) "Hosc". wp_auto.
+  wp_apply (wp_Select1 with "[Hosc]"). all: try done.
   {
-    done.
+   rewrite -> bool_decide_true by (apply n).
+   iFrame.
   }
-  {
-    iFrame.
-  }
-  iIntros (selected_idx) "Hosc".
-  wp_auto. 
+  iIntros (selected_idx) "Hosc". wp_auto.
   destruct selected_idx.
   {
-   simpl. 
-   unfold own_select_case. 
+    simpl. unfold own_select_case.
     iApply "HΦ". iFrame.
     destruct bool_decide.
-    {
-      iDestruct "Hosc" as "[Ht Hf]".
-      done.
-    } unfold own_select_case_logical.
-    iNamed "Hosc".
-    iFrame.
-    iNamed "Hosc". iFrame.
+    - iDestruct "Hosc" as "[Ht Hf]". done.
+    - unfold own_select_case_logical. iNamed "Hosc". iFrame. iNamed "Hosc". iFrame.
   }
-  iApply "HΦ".
-  unfold own_select_case.
-  destruct bool_decide eqn: Hb.
-  {
-    rewrite bool_decide_eq_true in Hb.
-    done.
-  }
-  iNamed "Hosc".
-  iDestruct "Hb" as "%". done.
+  iApply "HΦ". unfold own_select_case.
+  destruct bool_decide eqn:Hb.
+  - rewrite bool_decide_eq_true in Hb. done.
+  - iNamed "Hosc". iDestruct "Hb" as "%". done.
 Qed.
 
-Lemma wp_Channel__Receive (params: chan) (i: nat):
-  (if params.(ch_is_single_party) then params.(ch_q) = 1%Qp else (params.(ch_q) < 1)%Qp) ->
-  let T' := params.(ch_T') in
-  let T := params.(ch_T) in
-  let IntoVal_inst := params.(ch_IntoVal) in
-  let IntoValTyped_inst := params.(ch_IntoValTyped) in
-  let Hbounded := params.(ch_Hbounded) in
-  {{{ is_pkg_init channel ∗ recv_pre params i }}}
-    params.(ch_loc) @ channel @ "Channel'ptr" @ "Receive" #T #()
-  {{{ (v: params.(ch_T')) (ok: bool), RET (#v, #ok);
-      recv_post params i ok v
-  }}}.
+(*---------------------------------------------------------------------------
+ User must unfold recv_post, see chan_spec_inv for definition and descriptions
+ of chan record components
+ ---------------------------------------------------------------------------*)
+Lemma wp_Channel__Receive
+  (V: Type) {K: IntoVal V} {t: go_type}
+  {H': IntoValTyped V t} {B: BoundedTypeSize t}
+  (params: chan V) (i: nat) (q: Qp) (Ri: nat -> iProp Σ):
+  {{{ is_pkg_init channel ∗ recv_pre V params q i Ri }}}
+    params.(ch_loc) @ channel @ "Channel'ptr" @ "Receive" #t #()
+  {{{ (v: V) (ok: bool), RET (#v, #ok);
+      recv_post V params q i ok v Ri }}}.
 Proof.
-  intros Hsp HT' HT Hiv_inst Hivt_inst Hb_inst. wp_start. wp_auto. iNamed "Hpre". wp_if_destruct;first contradiction. wp_auto. wp_apply (wp_NewRecvCase with "[HCh HQ c HRecvPerm]"). 
-  {
-    iFrame. iPureIntro. done.
-  }
-  iIntros (case_ptr) "Hosc". wp_auto. wp_apply (wp_Select1 with "[Hosc]"). all: try done.
-  iIntros (selected_idx) "Hosc".
-  wp_auto.
+  wp_start. wp_auto. iNamed "Hpre".
+  wp_if_destruct; first contradiction. wp_auto.
+  wp_apply (wp_NewRecvCase with "[HCh HQ c HRecvPerm]").
+  { iFrame. iPureIntro. done. }
+  iIntros (case_ptr) "Hosc". wp_auto.
+  wp_apply (wp_Select1 with "[Hosc]"). all: try done.
+  iIntros (selected_idx) "Hosc". wp_auto.
   iNamed "Hosc".
   destruct selected_idx.
   {
-   simpl. 
-   unfold own_select_case. 
-   iNamed "Hosc". 
-   destruct bool_decide.
-   {
-    done.
-   }
-   iFrame.
-   iNamed "Hosc".
- 
-   wp_auto. iApply "HΦ". iFrame.
+    simpl. unfold own_select_case.
+    iNamed "Hosc".
+    destruct bool_decide; [done|].
+    iFrame. iNamed "Hosc".
+    wp_auto. iApply "HΦ". iFrame.
   }
   iDestruct "Hb" as "%". done.
 Qed.
 
-Lemma wp_Channel__ReceiveDiscardOk (params: chan) (i: nat):
-  (if params.(ch_is_single_party) then params.(ch_q) = 1%Qp else (params.(ch_q) < 1)%Qp) ->
-  let T' := params.(ch_T') in
-  let T := params.(ch_T) in
-  let IntoVal_inst := params.(ch_IntoVal) in
-  let IntoValTyped_inst := params.(ch_IntoValTyped) in
-  let Hbounded := params.(ch_Hbounded) in
-  {{{ is_pkg_init channel ∗ recv_pre params i }}}
-    params.(ch_loc) @ channel @ "Channel'ptr" @ "ReceiveDiscardOk" #T #()
-  {{{ (v: params.(ch_T')) (ok: bool), RET #v;
-      recv_post params i ok v
-  }}}.
+(*---------------------------------------------------------------------------
+Use if we don't use the ok value in a select case
+ ---------------------------------------------------------------------------*)
+Lemma wp_Channel__ReceiveDiscardOk
+  (V: Type) {K: IntoVal V} {t: go_type}
+  {H': IntoValTyped V t} {B: BoundedTypeSize t}
+  (params: chan V) (i: nat) (q: Qp) (Ri: nat -> iProp Σ):
+  {{{ is_pkg_init channel ∗ recv_pre V params q i Ri }}}
+    params.(ch_loc) @ channel @ "Channel'ptr" @ "ReceiveDiscardOk" #t #()
+  {{{ (v: V) (ok: bool), RET #v;
+      recv_post V params q i ok v Ri }}}.
 Proof.
-  intros Hsp HT' HT Hiv_inst Hivt_inst Hb_inst. wp_start. wp_auto. iNamed "Hpre".
+  wp_start. wp_auto. iNamed "Hpre".
   wp_apply (wp_Channel__Receive with "[HRecvPerm HQ HCh c]").
-  {
-    done.
-  }
-  {
-   iFrame. iPureIntro. done. 
-  }
+  { iFrame. done. }
   iIntros (v ok) "Hrcvpost". wp_auto. iApply "HΦ". done.
 Qed.
 
-Lemma wp_NewChannelRef
- (t': Type)
-  (t: go_type)
-(iv: IntoVal t')
-(ivt: IntoValTyped t' t)
-(hb: BoundedTypeSize t)
-(Psingle: Z -> t' -> iProp Σ)
-(size: Z)
-
-:
- 0 ≤ size ->
+(*--------------------------------------------------------------------------
+  This is the new specification that allows for choosing any of the available parameters. 
+  It is likely to be rare that all of these will be necessary but other specifications 
+  depend on this one. 
+ ---------------------------------------------------------------------------*)
+Lemma wp_NewChannelRef_base
+  (V: Type) {K: IntoVal V} {t: go_type} {H': IntoValTyped V t} {B: BoundedTypeSize t}
+  (size: Z)
+  (is_single_party: bool)
+  (Psingle: Z -> V -> iProp Σ)
+  (Pmulti: V -> iProp Σ)
+  (Qsingle: Z -> iProp Σ)
+  (Qmulti: iProp Σ)
+  (R: nat -> iProp Σ):
+  0 ≤ size ->
+  size + 1 < 2 ^ 63 ->
   {{{ is_pkg_init channel }}}
-    channel @ "NewChannelRef" #t #(W64 0)
-  {{{ (ch_ref_ptr: loc), RET #ch_ref_ptr;
-  ∃ (params:chan),
-          "%Hsize" ∷ ⌜params.(ch_size) = 0 ⌝ ∗ 
-          "%Hchptr" ∷ ⌜params.(ch_loc) = ch_ref_ptr⌝ ∗
-          "%Hchq" ∷ ⌜params.(ch_q) = 1%Qp⌝  ∗
-          "HCh" ∷ isChan params ∗ 
-          "HSc" ∷ own_send_counter_frag params.(ch_names) 0%nat params.(ch_q) ∗ 
-          "HRecvPerm" ∷ own_recv_perm params.(ch_names) params.(ch_q) 0 params.(ch_Ri)
+    channel @ "NewChannelRef" #t #(W64 size)
+  {{{ (ch_ref_ptr ch_mu_loc: loc) (ch_buff_slice: slice.t) (ch_γ_names: chan_names) (params: chan V),
+      RET #ch_ref_ptr;
+        "Hparams" ∷ ⌜params = {| ch_t := t;
+                                  ch_IntoVal := K;
+                                  ch_IntoValTyped := H';
+                                  ch_BoundedTypeSize := B;
+                                  ch_loc := ch_ref_ptr;
+                                  ch_mu := ch_mu_loc;
+                                  ch_buff := ch_buff_slice;
+                                  ch_γ := ch_γ_names;
+                                  ch_size := size;
+                                  ch_is_single_party := is_single_party;
+                                  ch_Psingle := Psingle;
+                                  ch_Pmulti := Pmulti;
+                                  ch_Qsingle := Qsingle;
+                                  ch_Qmulti := Qmulti;
+                                  ch_R := R |}⌝ ∗
+        "HCh" ∷ isChan V params ∗
+        own_closed_tok_auth params.(ch_γ) R ∗
+        "HSc" ∷ own_send_counter_frag params.(ch_γ) 0%nat 1 ∗
+        "HRecvPerm" ∷ own_recv_perm params.(ch_γ) 1 0 R
   }}}.
 Proof.
-  intros Hsz.
-   wp_start. wp_auto.
+  intros Hsz0 Hszlim.
+  wp_start. wp_auto.
   rewrite -wp_fupd.
-  wp_apply wp_slice_make2.
+  wp_apply ( @wp_slice_make2 _ _ _ _ _ _ V).
   iIntros (slice) "Hslice".
   wp_auto.
-  wp_alloc mu as "Hl".
+  wp_alloc mu as "Hmu".
   wp_auto.
   rewrite /named.
   wp_alloc loc as "HCh".
-
   iDestruct (struct_fields_split with "HCh") as "HCh".
   iNamed "HCh". simpl.
-  iDestruct own_chan_ghost_alloc as ">H".
-  iNamed "H".
-  iDestruct "H" as "(Hscauth & Hscf & Hrcauth & Hrperm & Hoct &Het)".
-  pose my_params := make_unbuffered_params_simple_single_sync t' t iv ivt hb loc mu slice γ Psingle
-  .
+  iDestruct own_chan_ghost_alloc as ">Hghost".
+  iNamed "Hghost".
+  iDestruct "Hghost" as "(Hscauth & Hscf & Hrcauth & Hrperm & Hoct &Het)".
+
+  (* Setup mutex and slice ownerships *)
   iPersist "Hlock" as "#mu".
   iPersist "Hbuffer" as "#buff".
-    
-
   iDestruct "Hslice" as "[Hsl1 Hsl2]".
   iDestruct (own_slice_len with "Hsl1") as "%Hlen".
 
-  iMod (init_Mutex (isChanInner my_params) _ mu
-         with "[$] [-HΦ Hscf Hrperm]") as "#Hlock".
-         {
-iModIntro.
-  unfold isChan. iFrame.
-  iFrame "#". 
-  unfold isChan. iFrame.
-  iFrame "#".
-  unfold make_unbuffered_params_simple_single_sync in my_params.
-  simpl in my_params.
-    replace my_params.(ch_buff) with slice in Hlen by done.
-  replace (my_params.(ch_size)) with 0 by set_solver.
-  simpl. rewrite length_replicate in Hlen.
-   replace (W64 0) with (slice .(slice.len_f)) by word.
-   iExists Valid_start. iFrame. iExists 0%nat.
-   replace (slice.(slice.len_f)) with (W64 0) by word.
-   iFrame. unfold isUnbufferedChan.
-   unfold chan_state_resources.
-   unfold chan_state_facts. simpl. 
-   iFrame.
-   done.
-  }
+  assert (size = uint.nat slice.(slice.len_f)).
+  { rewrite length_replicate in Hlen. rewrite <- Hlen. word. }
 
-  wp_auto_lc 2.
-  iModIntro.
-  iApply "HΦ".
-  replace mu with (my_params.(ch_mu)) by set_solver.
-  replace slice with (my_params.(ch_buff)) by set_solver.
-  iFrame "#".
-  replace (my_params.(ch_size)) with 0 by set_solver.
-  simpl. 
-  rewrite length_replicate in Hlen.
-    replace my_params.(ch_buff) with slice in Hlen by done.
-   replace (W64 0) with (slice .(slice.len_f)) by word.
-  iSplitL "".
+  iMod (init_Mutex (isChanInner V {|
+    ch_t := t;
+    ch_IntoVal := K;
+    ch_IntoValTyped := H';
+    ch_BoundedTypeSize := B;
+    ch_loc := loc;
+    ch_mu := mu;
+    ch_buff := slice;
+    ch_γ := γ;
+    ch_size := size;
+    ch_is_single_party := is_single_party;
+    ch_Psingle := Psingle;
+    ch_Pmulti := Pmulti;
+    ch_Qsingle := Qsingle;
+    ch_Qmulti := Qmulti;
+    ch_R := R
+  |}) _ mu with "[$] [-HΦ Hscf Hrperm Hoct]") as "#Hlock".
   {
-   done. 
+    iModIntro. unfold isChan. iFrame. iExists Valid_start.
+    iFrame "#". 
+    destruct (size =? 0) eqn:Hb.
+    - rewrite Hb. iFrame. iExists 0%nat. iFrame. done.
+    - rewrite Hb. iFrame. iExists 0%nat. unfold isBufferedChanLogical. iFrame "Hcount".
+      do 1 (iSplitL ""; first done). simpl. iFrame.
+      rewrite length_replicate in Hlen. rewrite length_replicate.
+      iFrame "%". iSplitL "";first word.
+      iAssert (big_sep_seq 0 0 (λ i,Q V is_single_party
+    (i - size - 1) Qsingle
+    Qmulti)) as "Hnil".
+    {
+      iApply big_sep_seq_nil. done.
+    }
+
+    iDestruct (big_sepL_intro (λ i,(λ i,Q V  is_single_party
+    (i - size) Qsingle
+    Qmulti)) (seqZ 0 (size)%Z)) as "H".
+    iAssert ([∗ list] x ∈ seqZ 0%nat (size), Q V is_single_party (x - size )
+      Qsingle Qmulti)%I with "[H]" as "HQs".
+    {
+      iApply "H". iIntros (k x). iIntros "%Hseq".
+      rewrite -> (lookup_seqZ 0 (size) k x) in Hseq.
+      destruct Hseq as [Hs1 Hs2].  subst x.
+       destruct k.
+      { unfold Q. assert (0 ≤  size). { lia. }
+        rewrite bool_decide_true. { done. } { lia. } }
+        unfold Q. rewrite bool_decide_true.
+        { done. }
+      lia.
+    }
+    unfold big_sep_seq. 
+    iFrame.
+    replace (size - 0%nat) with size by lia.
+    iFrame "HQs".
+    simpl. 
+   unfold valid_elems.
+    
+   iSplitL "". { iPureIntro. do 2 (split;first (try word;try done)).
+    {
+      inversion Hlen.
+      rewrite H. 
+      word.
+    }
+   }
+    replace (uint.nat (W64 0)) with 0%nat by word.
+    replace (uint.nat (W64 (Z.of_nat 0))) with 0%nat by word. simpl.
+    done.
+   }
+  {
+    wp_auto. iApply "HΦ". iFrame.
+    iSplitL ""; first done.
+    iFrame "#". simpl. iFrame. iPureIntro. rewrite H.
+    split.
+    { rewrite length_replicate in Hlen. rewrite <- H. inversion Hlen.
+      replace (slice.(slice.len_f)) with (W64 size) by word. done. }
+    word.
   }
-  iFrame.
-  iPureIntro. 
-   done.
 Qed.
 
-(* Len *)
-Lemma wp_Channel__Len_params (params: chan):
-  {{{ is_pkg_init channel ∗  isChan params }}}
-    params.(ch_loc) @ channel @ "Channel'ptr" @ "Len" #params.(ch_T) #()
+(*
+  Used for a simple sync use case where an unbuffered channel is used as a notfication or 
+  join handle. 
+*)
+Lemma wp_NewChannelRef_simple_unbuffered_sync
+(V: Type) {K: IntoVal V} {t: go_type} {H': IntoValTyped V t} {B: BoundedTypeSize t} 
+(Psingle: Z -> V -> iProp Σ):
+  {{{ is_pkg_init channel }}}
+    channel @ "NewChannelRef" #t #(W64 0)
+  {{{ (ch_ref_ptr: loc) (ch_mu_loc: loc) (ch_buff_slice: slice.t) (ch_γ_names: chan_names)  (params: chan V), RET #ch_ref_ptr;
+          "%Hparams" ∷ ⌜params = {|
+      ch_t := t;
+      ch_IntoVal := K;
+      ch_IntoValTyped := H';
+      ch_BoundedTypeSize := B;
+      ch_loc := ch_ref_ptr;
+      ch_mu := ch_mu_loc;
+      ch_buff := ch_buff_slice;
+      ch_γ := ch_γ_names;
+      ch_size := 0;
+      ch_is_single_party := true;
+      ch_Psingle := Psingle;  
+      ch_Pmulti := λ _, True%I;    
+      ch_Qsingle := λ _, True%I;   
+      ch_Qmulti := True%I;         
+      ch_R := λ _,False%I; (*No closing*)
+    |}⌝ ∗
+          "HCh" ∷ isChan V params ∗ 
+          "HSc" ∷ own_send_counter_frag ch_γ_names 0%nat 1 ∗ 
+          "HRecvPerm" ∷ own_recv_perm ch_γ_names 1 0 (λ _,False%I)
+  }}}.
+Proof.
+  wp_start_folded as "Hs".
+  wp_apply (((wp_NewChannelRef_base V 0 true Psingle (λ _, True%I) (λ _, True%I) (True%I) 
+  (λ _, False%I)) )). all: try done.
+  iIntros (ch_ref_ptr ch_mu_loc ch_buff_slice ch_γ_names params) "IH".
+  iNamed "IH". iDestruct "IH" as "(Hoct & HSc & HRecvPerm)".
+  iSpecialize ("HΦ" $! ch_ref_ptr ch_mu_loc ch_buff_slice ch_γ_names params). iApply "HΦ".
+  iDestruct "Hparams" as "%Hparams".
+  iFrame. subst. iFrame. iPureIntro. set_solver.
+Qed.
+  
+Lemma wp_Channel__Len (V: Type) {K: IntoVal V} {t: go_type} {H': IntoValTyped V t} {B: BoundedTypeSize t}  (params: chan V) :
+  {{{ is_pkg_init channel ∗  isChan V params }}}
+    params.(ch_loc) @ channel @ "Channel'ptr" @ "Len" #t #()
   {{{ (n: nat), RET #(W64 n); ⌜ (0 ≤ n)%nat ⌝ }}}.
 Proof.
   wp_start. wp_auto. iNamed "Hpre".  wp_if_destruct.
@@ -246,11 +326,10 @@ Proof.
   - iApply "HΦ". iPureIntro. lia.
 Qed.
 
-(* Cap *)
-Lemma wp_Channel__Cap_params (params: chan):
+Lemma wp_Channel__Cap (V: Type) {K: IntoVal V} {t: go_type} {H': IntoValTyped V t} {B: BoundedTypeSize t}  (params: chan V) :
   params.(ch_loc) ≠ null ->
-  {{{ is_pkg_init channel ∗ isChan params }}}
-    params.(ch_loc) @ channel @ "Channel'ptr" @ "Cap" #params.(ch_T) #()
+  {{{ is_pkg_init channel ∗ isChan V params }}}
+    params.(ch_loc) @ channel @ "Channel'ptr" @ "Cap" #t #()
   {{{ RET #(W64 params.(ch_size)); True%I }}}.
 Proof.
   intros Hnn.
@@ -271,12 +350,10 @@ Proof.
   }
 Qed.
 
-
-(* Close *)
-Lemma wp_Channel__Close (params: chan) (n: nat) :
+Lemma wp_Channel__Close (V: Type) {K: IntoVal V} {t: go_type} {H': IntoValTyped V t} {B: BoundedTypeSize t}  (params: chan V)  (n: nat) :
   #params.(ch_loc) ≠ #null ->
-  {{{ is_pkg_init channel ∗ "HCh" ∷ isChan params ∗ "HCp" ∷ own_close_perm params.(ch_names) params.(ch_R) n }}}
-    params.(ch_loc) @ channel @ "Channel'ptr" @ "Close" #params.(ch_T) #()
+  {{{ is_pkg_init channel ∗ "HCh" ∷ isChan V params ∗ "HCp" ∷ own_close_perm params.(ch_γ) params.(ch_R) n }}}
+    params.(ch_loc) @ channel @ "Channel'ptr" @ "Close" #t #()
   {{{ RET #(); True }}}.
 Proof.
   intros Hnotnull. wp_start. wp_auto.
@@ -290,8 +367,8 @@ Proof.
   iAssert (∃ (done_b: bool),
   "done" ∷  done_ptr ↦ done_b ∗ 
   if done_b then True else 
- ("HCh" ∷  isChan params ∗ 
-"HCp" ∷  own_close_perm params .(ch_names) params .(ch_R) n ∗ 
+ ("HCh" ∷  isChan V params ∗ 
+"HCp" ∷  own_close_perm params .(ch_γ) params .(ch_R) n ∗ 
 "c" ∷  c_ptr ↦ params .(ch_loc) )%I )%I
  with "[done HCh HCp c]" as "HI".
  {
@@ -377,41 +454,36 @@ Proof.
   }
 Qed.
 
-
 Lemma wp_Select2
-(params1 params2: chan) 
+(V1: Type) {K1: IntoVal V1} {t1: go_type} {H'1: IntoValTyped V1 t1} {B1: BoundedTypeSize t1}  (params1: chan V1)
+(V2: Type) {K2: IntoVal V2} {t2: go_type} {H'2: IntoValTyped V2 t2} {B2: BoundedTypeSize t2}  (params2: chan V2)
 (dir1 dir2: select_dir)
 (case1_ptr case2_ptr: loc)
 (i1 i2: nat) 
-(v1: params1.(ch_T')) (v2: params2.(ch_T'))
+(v1: V1) (v2: V2)
+(q1 q2: Qp)
+(Ri1 Ri2: nat-> iProp Σ)
 (blocking: bool):
-let T1 := params1.(ch_T) in
-let T2 := params2.(ch_T) in
-let IntoVal_inst1 := params1.(ch_IntoVal) in
-let IntoValTyped_inst1 := params1.(ch_IntoValTyped) in
-let IntoVal_inst2 := params2.(ch_IntoVal) in
-let IntoValTyped_inst2 := params2.(ch_IntoValTyped) in
 {{{ is_pkg_init channel ∗
-    own_select_case dir1 params1 case1_ptr false i1 #v1 ∗
-    own_select_case dir2 params2 case2_ptr false i2 #v2
+    own_select_case V1 params1 dir1 case1_ptr false i1 q1 #v1 Ri1 ∗
+    own_select_case V2 params2 dir2 case2_ptr false i2 q2 #v2 Ri2
 }}}
-  channel @ "Select2" #T1 #T2 #case1_ptr #case2_ptr #blocking
+  channel @ "Select2" #t1 #t2 #case1_ptr #case2_ptr #blocking
 {{{ (selected_idx: Z), RET #(W64 selected_idx);
     ⌜selected_idx ≤ 2⌝ ∗
     match selected_idx with 
     | 0 =>
-      own_select_case dir1 params1 case1_ptr true i1 #v1 ∗
-      own_select_case dir2 params2 case2_ptr false i2 #v2
+      own_select_case V1 params1 dir1 case1_ptr true i1 q1 #v1 Ri1 ∗
+      own_select_case V2 params2 dir2 case2_ptr false i2 q2 #v2 Ri2
     | 1 =>
-      own_select_case dir1 params1 case1_ptr false i1 #v1 ∗
-      own_select_case dir2 params2 case2_ptr true i2 #v2
+      own_select_case V1 params1 dir1 case1_ptr false i1 q1 #v1 Ri1 ∗
+      own_select_case V2 params2 dir2 case2_ptr true i2 q2 #v2 Ri2
     | _ => 
       ⌜blocking = false⌝ ∗
-      own_select_case dir1 params1 case1_ptr false i1 #v1 ∗
-      own_select_case dir2 params2 case2_ptr false i2 #v2
+      own_select_case V1 params1 dir1 case1_ptr false i1 q1 #v1 Ri1 ∗
+      own_select_case V2 params2 dir2 case2_ptr false i2 q2 #v2 Ri2
       end
 }}}.
-intros Ht1 Ht2 Hiv1 Hivt1 Hiv2 Hivt2.
 wp_start. wp_auto. 
 iNamed "Hpre". 
  wp_apply wp_alloc.
@@ -596,6 +668,5 @@ destruct selected.
 }
 }
 Qed.
-
 
 End proof.
